---
title: "1.2 Conservation Laws"
format:
    html:
        theme:
            light: flatly
            dark: darkly
        css: styles.css
        toc: true
---

Write a formula for the general solution of the equation $$u_t + cu_x = f(x)u$$

Answer

Assume $c$ a real valued constant, then we can do change of variables so that $U(\xi, \tau) = u(x,t)$ where
$$\xi = x - ct$$
$$\tau = t$$
Using chain rule, we got
$$u_t = U_\xi \xi_t + U_\tau \tau_t = U_\tau - cU_\xi$$
$$u_x = U_\xi \xi_x + U_\tau \tau_x = U_\xi$$
Substituting back to the original PDE will result in
$$U_\tau = f(\xi + c\tau)U$$
Solving this ODE with Factor of Integration will result in  
\begin{align*}
    e^{-\int f(\xi + c\tau) \; d\tau}f(\xi+\tau)U & = h(\xi) \\
    U &  = \frac{h(\xi)}{f(\xi+\tau)}e^{\int f(\xi + c\tau) \; d\tau} \\
    u(x,t) & = \frac{h(x - ct)}{f(x)} e^{\int \; f(x) dt}
\end{align*}