---
title: "1.2.8"
format:
    html:
        theme:
            light: flatly
            dark: darkly
        css: styles.css
        toc: true
---
                                          
Solve the pure initial value problem
$$u_t + u_x - 3u = t, \; x \in \mathbb{R}, \; t > 0$$
$$u(x,0) = x^2, \; x \in \mathbb{R}$$

Answer

Let $\xi = x - t$, $\tau = t$, and $U(\xi, \tau) = u(x,t)$ . By chain rule we have 
$$u_x = U_\xi \xi_x + U_\tau \tau_x =   U_\xi$$
$$u_t = U_\xi \xi_t + U_\tau \tau_t = U_\tau - U_\xi$$
Substituting all the changes to the original PDE, we have $$U_\tau - 3U = \tau$$
Integrating factor of above ODE is given by $$e^{\int -3 \;d\tau} = e^{-3\tau}$$
Thus by multiplying the ODE with integrating factor we got
\begin{align*}
    e^{-3\tau}U_\tau - 3e^{-3\tau}U & = e^{-3\tau}\tau \\
    \frac{d}{d\tau}(e^{-3\tau}U) & = e^{-3\tau}\tau \\
    e^{-3\tau}U = \int e^{-3\tau}\tau \; d\tau
\end{align*}
Using partial integral we will obtain that $$\int e^{-3\tau}\tau \; d\tau = -\frac{\tau e^{-3\tau}}{3} + \frac{1}{3}\int e^{-3\tau} \; d\tau = -\frac{\tau e^{-3\tau}}{3} - \frac{e^{-3\tau}}{9} + h(\xi)$$
Therefore $$U(\xi, \tau) = -\frac{\tau}{3} - \frac{1}{9} + h(\xi)e^{3\tau}$$

Changing back our variable to $t$ and $x$ will result in $$u(x, t) = - \frac{t}{3} - \frac{1}{9} + h(x - t)e^{3t}$$
If we apply the initial condition, then \begin{align*}
    x^2 = h(x) - \frac{1}{9} \\
    h(x) = x^2 + \frac{1}{9}
\end{align*}
Therefore our solution is $$u(x, t) = -\frac{t}{3} - \frac{1}{9} +  ((x-t)^2 + \frac{1}{9})e^{3t}$$